proofs/fstar/extraction/Polytune.Faand.fst
@@ -28,6 +28,25 @@ type t_Error =
   | Error_InvalidHashLength : t_Error
   | Error_OtErr : Polytune.Swankyot.t_Error -> t_Error
 
+/// Represents a cryptographic commitment as a fixed-size 32-byte array (a BLAKE3 hash).
+type t_Commitment = | Commitment : t_Array u8 (mk_usize 32) -> t_Commitment
+
+/// Commits to a value using the BLAKE3 cryptographic hash function.
+/// This is not a general-purpose commitment scheme, the input value is assumed to have high entropy.
+assume
+val commit': value: t_Slice u8 -> t_Commitment
+
+unfold
+let commit = commit'
+
+/// Verifies if a given value matches a previously generated commitment.
+/// This is not a general-purpose commitment scheme, the input value is assumed to have high entropy.
+assume
+val open_commitment': commitment: t_Commitment -> value: t_Slice u8 -> bool
+
+unfold
+let open_commitment = open_commitment'
+
 assume
 val lsb_of_hash__lsb_of_hash_inner': input: u128 -> bool
 
@@ -71,11 +90,1228 @@ let compute_hash_pointwise
   <:
   (bool & bool)
 
+let fhaand_compute_hashes
+      (delta: Polytune.Data_types.t_Delta)
+      (i n: usize)
+      (xshare: Polytune.Data_types.t_Share)
+      (yi: bool)
+      (randomness: t_Slice bool)
+    : Prims.Pure (Alloc.Vec.t_Vec (bool & bool) Alloc.Alloc.t_Global)
+      (requires
+        b2t
+        ((Alloc.Vec.impl_1__len #Polytune.Data_types.t_Key
+              #Alloc.Alloc.t_Global
+              (Polytune.Data_types.impl_Auth__keys xshare.Polytune.Data_types._1
+                <:
+                Alloc.Vec.t_Vec Polytune.Data_types.t_Key Alloc.Alloc.t_Global)
+            <:
+            usize) >=.
+          n
+          <:
+          bool) /\ b2t ((Core.Slice.impl__len #bool randomness <: usize) >=. n <: bool))
+      (ensures
+        fun result ->
+          let result:Alloc.Vec.t_Vec (bool & bool) Alloc.Alloc.t_Global = result in
+          b2t
+          ((Alloc.Vec.impl_1__len #(bool & bool) #Alloc.Alloc.t_Global result <: usize) =. n <: bool
+          )) =
+  let h0h1:Alloc.Vec.t_Vec (bool & bool) Alloc.Alloc.t_Global =
+    Alloc.Vec.from_elem #(bool & bool) (false, false <: (bool & bool)) n
+  in
+  Rust_primitives.Hax.Folds.fold_range (mk_usize 0)
+    n
+    (fun h0h1 temp_1_ ->
+        let h0h1:Alloc.Vec.t_Vec (bool & bool) Alloc.Alloc.t_Global = h0h1 in
+        let _:usize = temp_1_ in
+        b2t
+        ((Alloc.Vec.impl_1__len #(bool & bool) #Alloc.Alloc.t_Global h0h1 <: usize) =. n <: bool))
+    h0h1
+    (fun h0h1 j ->
+        let h0h1:Alloc.Vec.t_Vec (bool & bool) Alloc.Alloc.t_Global = h0h1 in
+        let j:usize = j in
+        if j =. i <: bool
+        then h0h1
+        else
+          let key_xj:Polytune.Data_types.t_Key = Polytune.Data_types.key_for xshare j in
+          let s_j:bool = randomness.[ j ] in
+          let h0, h1:(bool & bool) = compute_hash_pointwise delta yi key_xj s_j in
+          let h0h1:Alloc.Vec.t_Vec (bool & bool) Alloc.Alloc.t_Global =
+            Rust_primitives.Hax.Monomorphized_update_at.update_at_usize h0h1
+              j
+              ({ (h0h1.[ j ] <: (bool & bool)) with _1 = h0 } <: (bool & bool))
+          in
+          Rust_primitives.Hax.Monomorphized_update_at.update_at_usize h0h1
+            j
+            ({ (h0h1.[ j ] <: (bool & bool)) with _2 = h1 } <: (bool & bool)))
+
 let compute_t_pointwise (x_i: bool) (mac_by_j: Polytune.Data_types.t_Mac) (h0h1_j: (bool & bool))
     : bool =
   if x_i
   then Core.Ops.Bit.f_bitxor h0h1_j._2 (lsb_of_hash #Polytune.Data_types.t_Mac mac_by_j <: bool)
   else Core.Ops.Bit.f_bitxor h0h1_j._1 (lsb_of_hash #Polytune.Data_types.t_Mac mac_by_j <: bool)
+
+/// This function takes a 128-bit unsigned integer (`u128`) as input and produces a 128-bit hash value.
+/// We use the BLAKE3 cryptographic hash function to hash the input value and return the resulting hash.
+/// The hash is truncated to 128 bits to match the input size. Due to the truncation, the security
+/// guarantees of the hash function are reduced to 64-bit collision resistance and 128-bit preimage
+/// resistance. This is sufficient for the purposes of the protocol if RHO <= 64, which we expect
+/// to be the case in all real-world usages of our protocol.
+assume
+val hash128': input: u128 -> u128
+
+unfold
+let hash128 = hash128'
+
+let flaand_1_
+      (delta: Polytune.Data_types.t_Delta)
+      (xshares yshares rshares zshares: t_Slice Polytune.Data_types.t_Share)
+      (i n l: usize)
+      (v: Alloc.Vec.t_Vec bool Alloc.Alloc.t_Global)
+    : Prims.Pure
+      (t_Slice Polytune.Data_types.t_Share &
+        Core.Result.t_Result
+          (Alloc.Vec.t_Vec (Alloc.Vec.t_Vec u128 Alloc.Alloc.t_Global) Alloc.Alloc.t_Global &
+            Alloc.Vec.t_Vec (Alloc.Vec.t_Vec (bool & u128) Alloc.Alloc.t_Global)
+              Alloc.Alloc.t_Global &
+            Alloc.Vec.t_Vec u128 Alloc.Alloc.t_Global) t_Error)
+      (requires
+        b2t ((Alloc.Vec.impl_1__len #bool #Alloc.Alloc.t_Global v <: usize) >=. l <: bool) /\
+        b2t ((Core.Slice.impl__len #Polytune.Data_types.t_Share zshares <: usize) >=. l <: bool) /\
+        (b2t ((Core.Slice.impl__len #Polytune.Data_types.t_Share rshares <: usize) >=. l <: bool) /\
+        (b2t ((Core.Slice.impl__len #Polytune.Data_types.t_Share xshares <: usize) >=. l <: bool) /\
+        (forall (ll: usize).
+            b2t
+            ((mk_usize 0 <=. ll <: bool) && (ll <. l <: bool) &&
+              ((Core.Slice.impl__len #Polytune.Data_types.t_Share xshares <: usize) >=. l <: bool)) ==>
+            b2t
+            ((Alloc.Vec.impl_1__len #(Polytune.Data_types.t_Mac & Polytune.Data_types.t_Key)
+                  #Alloc.Alloc.t_Global
+                  (xshares.[ ll ] <: Polytune.Data_types.t_Share).Polytune.Data_types._1
+                    .Polytune.Data_types._0
+                <:
+                usize) >=.
+              n
+              <:
+              bool)) /\
+        (b2t ((Core.Slice.impl__len #Polytune.Data_types.t_Share yshares <: usize) >=. l <: bool) /\
+        (forall (ll: usize).
+            b2t
+            ((mk_usize 0 <=. ll <: bool) && (ll <. l <: bool) &&
+              ((Core.Slice.impl__len #Polytune.Data_types.t_Share yshares <: usize) >=. l <: bool)) ==>
+            b2t
+            ((Alloc.Vec.impl_1__len #(Polytune.Data_types.t_Mac & Polytune.Data_types.t_Key)
+                  #Alloc.Alloc.t_Global
+                  (yshares.[ ll ] <: Polytune.Data_types.t_Share).Polytune.Data_types._1
+                    .Polytune.Data_types._0
+                <:
+                usize) >=.
+              n
+              <:
+              bool))))))
+      (fun _ -> Prims.l_True) =
+  let z:Alloc.Vec.t_Vec bool Alloc.Alloc.t_Global = Alloc.Vec.from_elem #bool false l in
+  let e:Alloc.Vec.t_Vec bool Alloc.Alloc.t_Global = Alloc.Vec.from_elem #bool false l in
+  let e, z, zshares:(Alloc.Vec.t_Vec bool Alloc.Alloc.t_Global &
+    Alloc.Vec.t_Vec bool Alloc.Alloc.t_Global &
+    t_Slice Polytune.Data_types.t_Share) =
+    Rust_primitives.Hax.Folds.fold_range (mk_usize 0)
+      l
+      (fun temp_0_ temp_1_ ->
+          let e, z, zshares:(Alloc.Vec.t_Vec bool Alloc.Alloc.t_Global &
+            Alloc.Vec.t_Vec bool Alloc.Alloc.t_Global &
+            t_Slice Polytune.Data_types.t_Share) =
+            temp_0_
+          in
+          let _:usize = temp_1_ in
+          ((Alloc.Vec.impl_1__len #bool #Alloc.Alloc.t_Global z <: usize) =. l <: bool) &&
+          ((Alloc.Vec.impl_1__len #bool #Alloc.Alloc.t_Global e <: usize) =. l <: bool) &&
+          ((Core.Slice.impl__len #Polytune.Data_types.t_Share zshares <: usize) >=. l <: bool))
+      (e, z, zshares
+        <:
+        (Alloc.Vec.t_Vec bool Alloc.Alloc.t_Global & Alloc.Vec.t_Vec bool Alloc.Alloc.t_Global &
+          t_Slice Polytune.Data_types.t_Share))
+      (fun temp_0_ ll ->
+          let e, z, zshares:(Alloc.Vec.t_Vec bool Alloc.Alloc.t_Global &
+            Alloc.Vec.t_Vec bool Alloc.Alloc.t_Global &
+            t_Slice Polytune.Data_types.t_Share) =
+            temp_0_
+          in
+          let ll:usize = ll in
+          let z:Alloc.Vec.t_Vec bool Alloc.Alloc.t_Global =
+            Rust_primitives.Hax.Monomorphized_update_at.update_at_usize z
+              ll
+              (Core.Ops.Bit.f_bitxor (v.[ ll ] <: bool)
+                  (Core.Ops.Bit.f_bitand (xshares.[ ll ] <: Polytune.Data_types.t_Share)
+                        .Polytune.Data_types._0
+                      (yshares.[ ll ] <: Polytune.Data_types.t_Share).Polytune.Data_types._0
+                    <:
+                    bool)
+                <:
+                bool)
+          in
+          let e:Alloc.Vec.t_Vec bool Alloc.Alloc.t_Global =
+            Rust_primitives.Hax.Monomorphized_update_at.update_at_usize e
+              ll
+              (Core.Ops.Bit.f_bitxor (z.[ ll ] <: bool)
+                  (rshares.[ ll ] <: Polytune.Data_types.t_Share).Polytune.Data_types._0
+                <:
+                bool)
+          in
+          let zshares:t_Slice Polytune.Data_types.t_Share =
+            Rust_primitives.Hax.Monomorphized_update_at.update_at_usize zshares
+              ll
+              ({
+                  (zshares.[ ll ] <: Polytune.Data_types.t_Share) with
+                  Polytune.Data_types._0 = z.[ ll ] <: bool
+                }
+                <:
+                Polytune.Data_types.t_Share)
+          in
+          e, z, zshares
+          <:
+          (Alloc.Vec.t_Vec bool Alloc.Alloc.t_Global & Alloc.Vec.t_Vec bool Alloc.Alloc.t_Global &
+            t_Slice Polytune.Data_types.t_Share))
+  in
+  let phi:Alloc.Vec.t_Vec u128 Alloc.Alloc.t_Global = Alloc.Vec.from_elem #u128 (mk_u128 0) l in
+  let phi:Alloc.Vec.t_Vec u128 Alloc.Alloc.t_Global =
+    Rust_primitives.Hax.Folds.fold_range (mk_usize 0)
+      l
+      (fun phi temp_1_ ->
+          let phi:Alloc.Vec.t_Vec u128 Alloc.Alloc.t_Global = phi in
+          let _:usize = temp_1_ in
+          (Alloc.Vec.impl_1__len #u128 #Alloc.Alloc.t_Global phi <: usize) =. l <: bool)
+      phi
+      (fun phi ll ->
+          let phi:Alloc.Vec.t_Vec u128 Alloc.Alloc.t_Global = phi in
+          let ll:usize = ll in
+          let phi:Alloc.Vec.t_Vec u128 Alloc.Alloc.t_Global =
+            Rust_primitives.Hax.Folds.fold_range (mk_usize 0)
+              n
+              (fun phi temp_1_ ->
+                  let phi:Alloc.Vec.t_Vec u128 Alloc.Alloc.t_Global = phi in
+                  let _:usize = temp_1_ in
+                  (Alloc.Vec.impl_1__len #u128 #Alloc.Alloc.t_Global phi <: usize) =. l <: bool)
+              phi
+              (fun phi k ->
+                  let phi:Alloc.Vec.t_Vec u128 Alloc.Alloc.t_Global = phi in
+                  let k:usize = k in
+                  if k =. i <: bool
+                  then phi
+                  else
+                    let mk_yi, ki_yk:(Polytune.Data_types.t_Mac & Polytune.Data_types.t_Key) =
+                      (yshares.[ ll ] <: Polytune.Data_types.t_Share).Polytune.Data_types._1
+                        .Polytune.Data_types._0.[ k ]
+                    in
+                    let phi:Alloc.Vec.t_Vec u128 Alloc.Alloc.t_Global =
+                      Rust_primitives.Hax.Monomorphized_update_at.update_at_usize phi
+                        ll
+                        (((phi.[ ll ] <: u128) ^. ki_yk.Polytune.Data_types._0 <: u128) ^.
+                          mk_yi.Polytune.Data_types._0
+                          <:
+                          u128)
+                    in
+                    phi)
+          in
+          let phi:Alloc.Vec.t_Vec u128 Alloc.Alloc.t_Global =
+            Rust_primitives.Hax.Monomorphized_update_at.update_at_usize phi
+              ll
+              ((phi.[ ll ] <: u128) ^.
+                ((cast ((yshares.[ ll ] <: Polytune.Data_types.t_Share).Polytune.Data_types._0
+                        <:
+                        bool)
+                    <:
+                    u128) *!
+                  delta.Polytune.Data_types._0
+                  <:
+                  u128)
+                <:
+                u128)
+          in
+          phi)
+  in
+  let ki_xj_phi:Alloc.Vec.t_Vec (Alloc.Vec.t_Vec u128 Alloc.Alloc.t_Global) Alloc.Alloc.t_Global =
+    Alloc.Vec.from_elem #(Alloc.Vec.t_Vec u128 Alloc.Alloc.t_Global)
+      (Alloc.Vec.from_elem #u128 (mk_u128 0) l <: Alloc.Vec.t_Vec u128 Alloc.Alloc.t_Global)
+      n
+  in
+  let ei_uij:Alloc.Vec.t_Vec (Alloc.Vec.t_Vec (bool & u128) Alloc.Alloc.t_Global)
+    Alloc.Alloc.t_Global =
+    Alloc.Vec.from_elem #(Alloc.Vec.t_Vec (bool & u128) Alloc.Alloc.t_Global)
+      (Alloc.Vec.impl__new #(bool & u128) () <: Alloc.Vec.t_Vec (bool & u128) Alloc.Alloc.t_Global)
+      n
+  in
+  let ei_uij, ki_xj_phi:(Alloc.Vec.t_Vec (Alloc.Vec.t_Vec (bool & u128) Alloc.Alloc.t_Global)
+      Alloc.Alloc.t_Global &
+    Alloc.Vec.t_Vec (Alloc.Vec.t_Vec u128 Alloc.Alloc.t_Global) Alloc.Alloc.t_Global) =
+    Rust_primitives.Hax.Folds.fold_range (mk_usize 0)
+      n
+      (fun temp_0_ temp_1_ ->
+          let ei_uij, ki_xj_phi:(Alloc.Vec.t_Vec
+              (Alloc.Vec.t_Vec (bool & u128) Alloc.Alloc.t_Global) Alloc.Alloc.t_Global &
+            Alloc.Vec.t_Vec (Alloc.Vec.t_Vec u128 Alloc.Alloc.t_Global) Alloc.Alloc.t_Global) =
+            temp_0_
+          in
+          let _:usize = temp_1_ in
+          b2t
+          (((Alloc.Vec.impl_1__len #(Alloc.Vec.t_Vec u128 Alloc.Alloc.t_Global)
+                  #Alloc.Alloc.t_Global
+                  ki_xj_phi
+                <:
+                usize) =.
+              n
+              <:
+              bool) &&
+            ((Alloc.Vec.impl_1__len #(Alloc.Vec.t_Vec (bool & u128) Alloc.Alloc.t_Global)
+                  #Alloc.Alloc.t_Global
+                  ei_uij
+                <:
+                usize) =.
+              n
+              <:
+              bool) &&
+            ((Alloc.Vec.impl_1__len #u128 #Alloc.Alloc.t_Global phi <: usize) =. l <: bool)) /\
+          (forall (j: usize).
+              b2t
+              ((mk_usize 0 <=. j <: bool) && (j <. n <: bool) &&
+                ((Alloc.Vec.impl_1__len #(Alloc.Vec.t_Vec u128 Alloc.Alloc.t_Global)
+                      #Alloc.Alloc.t_Global
+                      ki_xj_phi
+                    <:
+                    usize) =.
+                  n
+                  <:
+                  bool)) ==>
+              b2t
+              ((Alloc.Vec.impl_1__len #u128
+                    #Alloc.Alloc.t_Global
+                    (ki_xj_phi.[ j ] <: Alloc.Vec.t_Vec u128 Alloc.Alloc.t_Global)
+                  <:
+                  usize) =.
+                l
+                <:
+                bool)))
+      (ei_uij, ki_xj_phi
+        <:
+        (Alloc.Vec.t_Vec (Alloc.Vec.t_Vec (bool & u128) Alloc.Alloc.t_Global) Alloc.Alloc.t_Global &
+          Alloc.Vec.t_Vec (Alloc.Vec.t_Vec u128 Alloc.Alloc.t_Global) Alloc.Alloc.t_Global))
+      (fun temp_0_ j ->
+          let ei_uij, ki_xj_phi:(Alloc.Vec.t_Vec
+              (Alloc.Vec.t_Vec (bool & u128) Alloc.Alloc.t_Global) Alloc.Alloc.t_Global &
+            Alloc.Vec.t_Vec (Alloc.Vec.t_Vec u128 Alloc.Alloc.t_Global) Alloc.Alloc.t_Global) =
+            temp_0_
+          in
+          let j:usize = j in
+          if j =. i <: bool
+          then
+            ei_uij, ki_xj_phi
+            <:
+            (Alloc.Vec.t_Vec (Alloc.Vec.t_Vec (bool & u128) Alloc.Alloc.t_Global)
+                Alloc.Alloc.t_Global &
+              Alloc.Vec.t_Vec (Alloc.Vec.t_Vec u128 Alloc.Alloc.t_Global) Alloc.Alloc.t_Global)
+          else
+            Rust_primitives.Hax.Folds.fold_range (mk_usize 0)
+              l
+              (fun temp_0_ temp_1_ ->
+                  let ei_uij, ki_xj_phi:(Alloc.Vec.t_Vec
+                      (Alloc.Vec.t_Vec (bool & u128) Alloc.Alloc.t_Global) Alloc.Alloc.t_Global &
+                    Alloc.Vec.t_Vec (Alloc.Vec.t_Vec u128 Alloc.Alloc.t_Global) Alloc.Alloc.t_Global
+                  ) =
+                    temp_0_
+                  in
+                  let _:usize = temp_1_ in
+                  b2t
+                  (((Alloc.Vec.impl_1__len #(Alloc.Vec.t_Vec u128 Alloc.Alloc.t_Global)
+                          #Alloc.Alloc.t_Global
+                          ki_xj_phi
+                        <:
+                        usize) =.
+                      n
+                      <:
+                      bool) &&
+                    ((Alloc.Vec.impl_1__len #(Alloc.Vec.t_Vec (bool & u128) Alloc.Alloc.t_Global)
+                          #Alloc.Alloc.t_Global
+                          ei_uij
+                        <:
+                        usize) =.
+                      n
+                      <:
+                      bool) &&
+                    ((Alloc.Vec.impl_1__len #u128 #Alloc.Alloc.t_Global phi <: usize) =. l <: bool)) /\
+                  (forall (j: usize).
+                      b2t
+                      ((mk_usize 0 <=. j <: bool) && (j <. n <: bool) &&
+                        ((Alloc.Vec.impl_1__len #(Alloc.Vec.t_Vec u128 Alloc.Alloc.t_Global)
+                              #Alloc.Alloc.t_Global
+                              ki_xj_phi
+                            <:
+                            usize) =.
+                          n
+                          <:
+                          bool)) ==>
+                      b2t
+                      ((Alloc.Vec.impl_1__len #u128
+                            #Alloc.Alloc.t_Global
+                            (ki_xj_phi.[ j ] <: Alloc.Vec.t_Vec u128 Alloc.Alloc.t_Global)
+                          <:
+                          usize) =.
+                        l
+                        <:
+                        bool)))
+              (ei_uij, ki_xj_phi
+                <:
+                (Alloc.Vec.t_Vec (Alloc.Vec.t_Vec (bool & u128) Alloc.Alloc.t_Global)
+                    Alloc.Alloc.t_Global &
+                  Alloc.Vec.t_Vec (Alloc.Vec.t_Vec u128 Alloc.Alloc.t_Global) Alloc.Alloc.t_Global))
+              (fun temp_0_ ll ->
+                  let ei_uij, ki_xj_phi:(Alloc.Vec.t_Vec
+                      (Alloc.Vec.t_Vec (bool & u128) Alloc.Alloc.t_Global) Alloc.Alloc.t_Global &
+                    Alloc.Vec.t_Vec (Alloc.Vec.t_Vec u128 Alloc.Alloc.t_Global) Alloc.Alloc.t_Global
+                  ) =
+                    temp_0_
+                  in
+                  let ll:usize = ll in
+                  let _, ki_xj:(Polytune.Data_types.t_Mac & Polytune.Data_types.t_Key) =
+                    (xshares.[ ll ] <: Polytune.Data_types.t_Share).Polytune.Data_types._1
+                      .Polytune.Data_types._0.[ j ]
+                  in
+                  let ki_xj_phi:Alloc.Vec.t_Vec (Alloc.Vec.t_Vec u128 Alloc.Alloc.t_Global)
+                    Alloc.Alloc.t_Global =
+                    Rust_primitives.Hax.Monomorphized_update_at.update_at_usize ki_xj_phi
+                      j
+                      (Rust_primitives.Hax.Monomorphized_update_at.update_at_usize (ki_xj_phi.[ j ]
+                            <:
+                            Alloc.Vec.t_Vec u128 Alloc.Alloc.t_Global)
+                          ll
+                          (hash128 ki_xj.Polytune.Data_types._0 <: u128)
+                        <:
+                        Alloc.Vec.t_Vec u128 Alloc.Alloc.t_Global)
+                  in
+                  let uij:u128 =
+                    ((hash128 (ki_xj.Polytune.Data_types._0 ^. delta.Polytune.Data_types._0 <: u128)
+                        <:
+                        u128) ^.
+                      ((ki_xj_phi.[ j ] <: Alloc.Vec.t_Vec u128 Alloc.Alloc.t_Global).[ ll ] <: u128
+                      )
+                      <:
+                      u128) ^.
+                    (phi.[ ll ] <: u128)
+                  in
+                  let ei_uij:Alloc.Vec.t_Vec (Alloc.Vec.t_Vec (bool & u128) Alloc.Alloc.t_Global)
+                    Alloc.Alloc.t_Global =
+                    Rust_primitives.Hax.Monomorphized_update_at.update_at_usize ei_uij
+                      j
+                      (Alloc.Vec.impl_1__push #(bool & u128)
+                          #Alloc.Alloc.t_Global
+                          (ei_uij.[ j ] <: Alloc.Vec.t_Vec (bool & u128) Alloc.Alloc.t_Global)
+                          ((e.[ ll ] <: bool), uij <: (bool & u128))
+                        <:
+                        Alloc.Vec.t_Vec (bool & u128) Alloc.Alloc.t_Global)
+                  in
+                  ei_uij, ki_xj_phi
+                  <:
+                  (Alloc.Vec.t_Vec (Alloc.Vec.t_Vec (bool & u128) Alloc.Alloc.t_Global)
+                      Alloc.Alloc.t_Global &
+                    Alloc.Vec.t_Vec (Alloc.Vec.t_Vec u128 Alloc.Alloc.t_Global) Alloc.Alloc.t_Global
+                  ))
+            <:
+            (Alloc.Vec.t_Vec (Alloc.Vec.t_Vec (bool & u128) Alloc.Alloc.t_Global)
+                Alloc.Alloc.t_Global &
+              Alloc.Vec.t_Vec (Alloc.Vec.t_Vec u128 Alloc.Alloc.t_Global) Alloc.Alloc.t_Global))
+  in
+  let hax_temp_output:Core.Result.t_Result
+    (Alloc.Vec.t_Vec (Alloc.Vec.t_Vec u128 Alloc.Alloc.t_Global) Alloc.Alloc.t_Global &
+      Alloc.Vec.t_Vec (Alloc.Vec.t_Vec (bool & u128) Alloc.Alloc.t_Global) Alloc.Alloc.t_Global &
+      Alloc.Vec.t_Vec u128 Alloc.Alloc.t_Global) t_Error =
+    Core.Result.Result_Ok
+    (ki_xj_phi, ei_uij, phi
+      <:
+      (Alloc.Vec.t_Vec (Alloc.Vec.t_Vec u128 Alloc.Alloc.t_Global) Alloc.Alloc.t_Global &
+        Alloc.Vec.t_Vec (Alloc.Vec.t_Vec (bool & u128) Alloc.Alloc.t_Global) Alloc.Alloc.t_Global &
+        Alloc.Vec.t_Vec u128 Alloc.Alloc.t_Global))
+    <:
+    Core.Result.t_Result
+      (Alloc.Vec.t_Vec (Alloc.Vec.t_Vec u128 Alloc.Alloc.t_Global) Alloc.Alloc.t_Global &
+        Alloc.Vec.t_Vec (Alloc.Vec.t_Vec (bool & u128) Alloc.Alloc.t_Global) Alloc.Alloc.t_Global &
+        Alloc.Vec.t_Vec u128 Alloc.Alloc.t_Global) t_Error
+  in
+  zshares, hax_temp_output
+  <:
+  (t_Slice Polytune.Data_types.t_Share &
+    Core.Result.t_Result
+      (Alloc.Vec.t_Vec (Alloc.Vec.t_Vec u128 Alloc.Alloc.t_Global) Alloc.Alloc.t_Global &
+        Alloc.Vec.t_Vec (Alloc.Vec.t_Vec (bool & u128) Alloc.Alloc.t_Global) Alloc.Alloc.t_Global &
+        Alloc.Vec.t_Vec u128 Alloc.Alloc.t_Global) t_Error)
+
+let flaand_2_
+      (delta: Polytune.Data_types.t_Delta)
+      (xshares rshares: t_Slice Polytune.Data_types.t_Share)
+      (i n l: usize)
+      (ki_xj_phi: Alloc.Vec.t_Vec (Alloc.Vec.t_Vec u128 Alloc.Alloc.t_Global) Alloc.Alloc.t_Global)
+      (ei_uij_k:
+          Alloc.Vec.t_Vec (Alloc.Vec.t_Vec (bool & u128) Alloc.Alloc.t_Global) Alloc.Alloc.t_Global)
+      (zshares: Alloc.Vec.t_Vec Polytune.Data_types.t_Share Alloc.Alloc.t_Global)
+      (phi: Alloc.Vec.t_Vec u128 Alloc.Alloc.t_Global)
+    : Prims.Pure
+      (Alloc.Vec.t_Vec (Alloc.Vec.t_Vec u128 Alloc.Alloc.t_Global) Alloc.Alloc.t_Global &
+        Alloc.Vec.t_Vec Polytune.Data_types.t_Share Alloc.Alloc.t_Global &
+        Core.Result.t_Result
+          (Alloc.Vec.t_Vec t_Commitment Alloc.Alloc.t_Global &
+            Alloc.Vec.t_Vec u128 Alloc.Alloc.t_Global) t_Error)
+      (requires
+        b2t ((Alloc.Vec.impl_1__len #u128 #Alloc.Alloc.t_Global phi <: usize) >=. l <: bool) /\
+        b2t ((Core.Slice.impl__len #Polytune.Data_types.t_Share rshares <: usize) >=. l <: bool) /\
+        (forall (ll: usize).
+            b2t
+            ((mk_usize 0 <=. ll <: bool) && (ll <. l <: bool) &&
+              ((Core.Slice.impl__len #Polytune.Data_types.t_Share rshares <: usize) >=. l <: bool)) ==>
+            b2t
+            ((Alloc.Vec.impl_1__len #(Polytune.Data_types.t_Mac & Polytune.Data_types.t_Key)
+                  #Alloc.Alloc.t_Global
+                  (rshares.[ ll ] <: Polytune.Data_types.t_Share).Polytune.Data_types._1
+                    .Polytune.Data_types._0
+                <:
+                usize) >=.
+              n
+              <:
+              bool)) /\
+        (b2t
+        ((Alloc.Vec.impl_1__len #Polytune.Data_types.t_Share #Alloc.Alloc.t_Global zshares <: usize) >=.
+          l
+          <:
+          bool) /\
+        (forall (ll: usize).
+            b2t
+            ((mk_usize 0 <=. ll <: bool) && (ll <. l <: bool) &&
+              ((Alloc.Vec.impl_1__len #Polytune.Data_types.t_Share #Alloc.Alloc.t_Global zshares
+                  <:
+                  usize) >=.
+                l
+                <:
+                bool)) ==>
+            b2t
+            ((Alloc.Vec.impl_1__len #(Polytune.Data_types.t_Mac & Polytune.Data_types.t_Key)
+                  #Alloc.Alloc.t_Global
+                  (zshares.[ ll ] <: Polytune.Data_types.t_Share).Polytune.Data_types._1
+                    .Polytune.Data_types._0
+                <:
+                usize) >=.
+              n
+              <:
+              bool)) /\
+        (b2t ((Core.Slice.impl__len #Polytune.Data_types.t_Share xshares <: usize) >=. l <: bool) /\
+        (forall (ll: usize).
+            b2t
+            ((mk_usize 0 <=. ll <: bool) && (ll <. l <: bool) &&
+              ((Core.Slice.impl__len #Polytune.Data_types.t_Share xshares <: usize) >=. l <: bool)) ==>
+            b2t
+            ((Alloc.Vec.impl_1__len #(Polytune.Data_types.t_Mac & Polytune.Data_types.t_Key)
+                  #Alloc.Alloc.t_Global
+                  (xshares.[ ll ] <: Polytune.Data_types.t_Share).Polytune.Data_types._1
+                    .Polytune.Data_types._0
+                <:
+                usize) >=.
+              n
+              <:
+              bool)))) /\
+        (b2t
+        ((Alloc.Vec.impl_1__len #(Alloc.Vec.t_Vec (bool & u128) Alloc.Alloc.t_Global)
+              #Alloc.Alloc.t_Global
+              ei_uij_k
+            <:
+            usize) >=.
+          n
+          <:
+          bool) /\
+        (forall (j: usize).
+            b2t
+            ((mk_usize 0 <=. j <: bool) && (j <. n <: bool) &&
+              ((Alloc.Vec.impl_1__len #(Alloc.Vec.t_Vec (bool & u128) Alloc.Alloc.t_Global)
+                    #Alloc.Alloc.t_Global
+                    ei_uij_k
+                  <:
+                  usize) >=.
+                n
+                <:
+                bool)) ==>
+            b2t
+            ((Alloc.Vec.impl_1__len #(bool & u128)
+                  #Alloc.Alloc.t_Global
+                  (ei_uij_k.[ j ] <: Alloc.Vec.t_Vec (bool & u128) Alloc.Alloc.t_Global)
+                <:
+                usize) >=.
+              l
+              <:
+              bool)) /\
+        (b2t
+        ((Alloc.Vec.impl_1__len #(Alloc.Vec.t_Vec u128 Alloc.Alloc.t_Global)
+              #Alloc.Alloc.t_Global
+              ki_xj_phi
+            <:
+            usize) >=.
+          n
+          <:
+          bool) /\
+        (forall (j: usize).
+            b2t
+            ((mk_usize 0 <=. j <: bool) && (j <. n <: bool) &&
+              ((Alloc.Vec.impl_1__len #(Alloc.Vec.t_Vec u128 Alloc.Alloc.t_Global)
+                    #Alloc.Alloc.t_Global
+                    ki_xj_phi
+                  <:
+                  usize) >=.
+                n
+                <:
+                bool)) ==>
+            b2t
+            ((Alloc.Vec.impl_1__len #u128
+                  #Alloc.Alloc.t_Global
+                  (ki_xj_phi.[ j ] <: Alloc.Vec.t_Vec u128 Alloc.Alloc.t_Global)
+                <:
+                usize) >=.
+              l
+              <:
+              bool)))))
+      (fun _ -> Prims.l_True) =
+  let ki_xj_phi, zshares:(Alloc.Vec.t_Vec (Alloc.Vec.t_Vec u128 Alloc.Alloc.t_Global)
+      Alloc.Alloc.t_Global &
+    Alloc.Vec.t_Vec Polytune.Data_types.t_Share Alloc.Alloc.t_Global) =
+    Rust_primitives.Hax.Folds.fold_range (mk_usize 0)
+      n
+      (fun temp_0_ temp_1_ ->
+          let ki_xj_phi, zshares:(Alloc.Vec.t_Vec (Alloc.Vec.t_Vec u128 Alloc.Alloc.t_Global)
+              Alloc.Alloc.t_Global &
+            Alloc.Vec.t_Vec Polytune.Data_types.t_Share Alloc.Alloc.t_Global) =
+            temp_0_
+          in
+          let _:usize = temp_1_ in
+          b2t
+          ((Alloc.Vec.impl_1__len #(Alloc.Vec.t_Vec u128 Alloc.Alloc.t_Global)
+                #Alloc.Alloc.t_Global
+                ki_xj_phi
+              <:
+              usize) >=.
+            n
+            <:
+            bool) /\
+          (forall (j: usize).
+              b2t
+              ((mk_usize 0 <=. j <: bool) && (j <. n <: bool) &&
+                ((Alloc.Vec.impl_1__len #(Alloc.Vec.t_Vec u128 Alloc.Alloc.t_Global)
+                      #Alloc.Alloc.t_Global
+                      ki_xj_phi
+                    <:
+                    usize) >=.
+                  n
+                  <:
+                  bool)) ==>
+              b2t
+              ((Alloc.Vec.impl_1__len #u128
+                    #Alloc.Alloc.t_Global
+                    (ki_xj_phi.[ j ] <: Alloc.Vec.t_Vec u128 Alloc.Alloc.t_Global)
+                  <:
+                  usize) >=.
+                l
+                <:
+                bool)) /\
+          b2t
+          ((Alloc.Vec.impl_1__len #Polytune.Data_types.t_Share #Alloc.Alloc.t_Global zshares
+              <:
+              usize) >=.
+            l
+            <:
+            bool) /\
+          (forall (ll: usize).
+              b2t
+              ((mk_usize 0 <=. ll <: bool) && (ll <. l <: bool) &&
+                ((Alloc.Vec.impl_1__len #Polytune.Data_types.t_Share #Alloc.Alloc.t_Global zshares
+                    <:
+                    usize) >=.
+                  l
+                  <:
+                  bool)) ==>
+              b2t
+              ((Alloc.Vec.impl_1__len #(Polytune.Data_types.t_Mac & Polytune.Data_types.t_Key)
+                    #Alloc.Alloc.t_Global
+                    (zshares.[ ll ] <: Polytune.Data_types.t_Share).Polytune.Data_types._1
+                      .Polytune.Data_types._0
+                  <:
+                  usize) >=.
+                n
+                <:
+                bool)))
+      (ki_xj_phi, zshares
+        <:
+        (Alloc.Vec.t_Vec (Alloc.Vec.t_Vec u128 Alloc.Alloc.t_Global) Alloc.Alloc.t_Global &
+          Alloc.Vec.t_Vec Polytune.Data_types.t_Share Alloc.Alloc.t_Global))
+      (fun temp_0_ j ->
+          let ki_xj_phi, zshares:(Alloc.Vec.t_Vec (Alloc.Vec.t_Vec u128 Alloc.Alloc.t_Global)
+              Alloc.Alloc.t_Global &
+            Alloc.Vec.t_Vec Polytune.Data_types.t_Share Alloc.Alloc.t_Global) =
+            temp_0_
+          in
+          let j:usize = j in
+          if j =. i <: bool
+          then
+            ki_xj_phi, zshares
+            <:
+            (Alloc.Vec.t_Vec (Alloc.Vec.t_Vec u128 Alloc.Alloc.t_Global) Alloc.Alloc.t_Global &
+              Alloc.Vec.t_Vec Polytune.Data_types.t_Share Alloc.Alloc.t_Global)
+          else
+            Rust_primitives.Hax.Folds.fold_range (mk_usize 0)
+              l
+              (fun temp_0_ temp_1_ ->
+                  let ki_xj_phi, zshares:(Alloc.Vec.t_Vec
+                      (Alloc.Vec.t_Vec u128 Alloc.Alloc.t_Global) Alloc.Alloc.t_Global &
+                    Alloc.Vec.t_Vec Polytune.Data_types.t_Share Alloc.Alloc.t_Global) =
+                    temp_0_
+                  in
+                  let _:usize = temp_1_ in
+                  b2t
+                  ((Alloc.Vec.impl_1__len #(Alloc.Vec.t_Vec u128 Alloc.Alloc.t_Global)
+                        #Alloc.Alloc.t_Global
+                        ki_xj_phi
+                      <:
+                      usize) >=.
+                    n
+                    <:
+                    bool) /\
+                  (forall (j: usize).
+                      b2t
+                      ((mk_usize 0 <=. j <: bool) && (j <. n <: bool) &&
+                        ((Alloc.Vec.impl_1__len #(Alloc.Vec.t_Vec u128 Alloc.Alloc.t_Global)
+                              #Alloc.Alloc.t_Global
+                              ki_xj_phi
+                            <:
+                            usize) >=.
+                          n
+                          <:
+                          bool)) ==>
+                      b2t
+                      ((Alloc.Vec.impl_1__len #u128
+                            #Alloc.Alloc.t_Global
+                            (ki_xj_phi.[ j ] <: Alloc.Vec.t_Vec u128 Alloc.Alloc.t_Global)
+                          <:
+                          usize) >=.
+                        l
+                        <:
+                        bool)) /\
+                  b2t
+                  ((Alloc.Vec.impl_1__len #Polytune.Data_types.t_Share #Alloc.Alloc.t_Global zshares
+                      <:
+                      usize) >=.
+                    l
+                    <:
+                    bool) /\
+                  (forall (ll: usize).
+                      b2t
+                      ((mk_usize 0 <=. ll <: bool) && (ll <. l <: bool) &&
+                        ((Alloc.Vec.impl_1__len #Polytune.Data_types.t_Share
+                              #Alloc.Alloc.t_Global
+                              zshares
+                            <:
+                            usize) >=.
+                          l
+                          <:
+                          bool)) ==>
+                      b2t
+                      ((Alloc.Vec.impl_1__len #(Polytune.Data_types.t_Mac &
+                              Polytune.Data_types.t_Key)
+                            #Alloc.Alloc.t_Global
+                            (zshares.[ ll ] <: Polytune.Data_types.t_Share).Polytune.Data_types._1
+                              .Polytune.Data_types._0
+                          <:
+                          usize) >=.
+                        n
+                        <:
+                        bool)))
+              (ki_xj_phi, zshares
+                <:
+                (Alloc.Vec.t_Vec (Alloc.Vec.t_Vec u128 Alloc.Alloc.t_Global) Alloc.Alloc.t_Global &
+                  Alloc.Vec.t_Vec Polytune.Data_types.t_Share Alloc.Alloc.t_Global))
+              (fun temp_0_ ll ->
+                  let ki_xj_phi, zshares:(Alloc.Vec.t_Vec
+                      (Alloc.Vec.t_Vec u128 Alloc.Alloc.t_Global) Alloc.Alloc.t_Global &
+                    Alloc.Vec.t_Vec Polytune.Data_types.t_Share Alloc.Alloc.t_Global) =
+                    temp_0_
+                  in
+                  let ll:usize = ll in
+                  let mi_xj, _:(Polytune.Data_types.t_Mac & Polytune.Data_types.t_Key) =
+                    (xshares.[ ll ] <: Polytune.Data_types.t_Share).Polytune.Data_types._1
+                      .Polytune.Data_types._0.[ j ]
+                  in
+                  let ki_xj_phi:Alloc.Vec.t_Vec (Alloc.Vec.t_Vec u128 Alloc.Alloc.t_Global)
+                    Alloc.Alloc.t_Global =
+                    Rust_primitives.Hax.Monomorphized_update_at.update_at_usize ki_xj_phi
+                      j
+                      (Rust_primitives.Hax.Monomorphized_update_at.update_at_usize (ki_xj_phi.[ j ]
+                            <:
+                            Alloc.Vec.t_Vec u128 Alloc.Alloc.t_Global)
+                          ll
+                          ((((ki_xj_phi.[ j ] <: Alloc.Vec.t_Vec u128 Alloc.Alloc.t_Global).[ ll ]
+                                <:
+                                u128) ^.
+                              (hash128 mi_xj.Polytune.Data_types._0 <: u128)
+                              <:
+                              u128) ^.
+                            ((cast ((xshares.[ ll ] <: Polytune.Data_types.t_Share)
+                                      .Polytune.Data_types._0
+                                    <:
+                                    bool)
+                                <:
+                                u128) *!
+                              ((ei_uij_k.[ j ] <: Alloc.Vec.t_Vec (bool & u128) Alloc.Alloc.t_Global
+                                ).[ ll ]
+                                <:
+                                (bool & u128))
+                                ._2
+                              <:
+                              u128)
+                            <:
+                            u128)
+                        <:
+                        Alloc.Vec.t_Vec u128 Alloc.Alloc.t_Global)
+                  in
+                  let mac, key:(Polytune.Data_types.t_Mac & Polytune.Data_types.t_Key) =
+                    (rshares.[ ll ] <: Polytune.Data_types.t_Share).Polytune.Data_types._1
+                      .Polytune.Data_types._0.[ j ]
+                  in
+                  if
+                    ((ei_uij_k.[ j ] <: Alloc.Vec.t_Vec (bool & u128) Alloc.Alloc.t_Global).[ ll ] <: (bool & u128))
+                      ._1
+                  then
+                    let zshares:Alloc.Vec.t_Vec Polytune.Data_types.t_Share Alloc.Alloc.t_Global =
+                      Rust_primitives.Hax.Monomorphized_update_at.update_at_usize zshares
+                        ll
+                        ({
+                            (zshares.[ ll ] <: Polytune.Data_types.t_Share) with
+                            Polytune.Data_types._1
+                            =
+                            {
+                              (zshares.[ ll ] <: Polytune.Data_types.t_Share).Polytune.Data_types._1 with
+                              Polytune.Data_types._0
+                              =
+                              Rust_primitives.Hax.Monomorphized_update_at.update_at_usize (zshares.[
+                                    ll ]
+                                  <:
+                                  Polytune.Data_types.t_Share)
+                                  .Polytune.Data_types._1
+                                  .Polytune.Data_types._0
+                                j
+                                (mac,
+                                  (Polytune.Data_types.Key
+                                    (key.Polytune.Data_types._0 ^. delta.Polytune.Data_types._0
+                                      <:
+                                      u128)
+                                    <:
+                                    Polytune.Data_types.t_Key)
+                                  <:
+                                  (Polytune.Data_types.t_Mac & Polytune.Data_types.t_Key))
+                              <:
+                              Alloc.Vec.t_Vec
+                                (Polytune.Data_types.t_Mac & Polytune.Data_types.t_Key)
+                                Alloc.Alloc.t_Global
+                            }
+                            <:
+                            Polytune.Data_types.t_Auth
+                          }
+                          <:
+                          Polytune.Data_types.t_Share)
+                    in
+                    ki_xj_phi, zshares
+                    <:
+                    (Alloc.Vec.t_Vec (Alloc.Vec.t_Vec u128 Alloc.Alloc.t_Global)
+                        Alloc.Alloc.t_Global &
+                      Alloc.Vec.t_Vec Polytune.Data_types.t_Share Alloc.Alloc.t_Global)
+                  else
+                    let zshares:Alloc.Vec.t_Vec Polytune.Data_types.t_Share Alloc.Alloc.t_Global =
+                      Rust_primitives.Hax.Monomorphized_update_at.update_at_usize zshares
+                        ll
+                        ({
+                            (zshares.[ ll ] <: Polytune.Data_types.t_Share) with
+                            Polytune.Data_types._1
+                            =
+                            {
+                              (zshares.[ ll ] <: Polytune.Data_types.t_Share).Polytune.Data_types._1 with
+                              Polytune.Data_types._0
+                              =
+                              Rust_primitives.Hax.Monomorphized_update_at.update_at_usize (zshares.[
+                                    ll ]
+                                  <:
+                                  Polytune.Data_types.t_Share)
+                                  .Polytune.Data_types._1
+                                  .Polytune.Data_types._0
+                                j
+                                (mac, key <: (Polytune.Data_types.t_Mac & Polytune.Data_types.t_Key)
+                                )
+                              <:
+                              Alloc.Vec.t_Vec
+                                (Polytune.Data_types.t_Mac & Polytune.Data_types.t_Key)
+                                Alloc.Alloc.t_Global
+                            }
+                            <:
+                            Polytune.Data_types.t_Auth
+                          }
+                          <:
+                          Polytune.Data_types.t_Share)
+                    in
+                    ki_xj_phi, zshares
+                    <:
+                    (Alloc.Vec.t_Vec (Alloc.Vec.t_Vec u128 Alloc.Alloc.t_Global)
+                        Alloc.Alloc.t_Global &
+                      Alloc.Vec.t_Vec Polytune.Data_types.t_Share Alloc.Alloc.t_Global))
+            <:
+            (Alloc.Vec.t_Vec (Alloc.Vec.t_Vec u128 Alloc.Alloc.t_Global) Alloc.Alloc.t_Global &
+              Alloc.Vec.t_Vec Polytune.Data_types.t_Share Alloc.Alloc.t_Global))
+  in
+  let hi:Alloc.Vec.t_Vec u128 Alloc.Alloc.t_Global = Alloc.Vec.from_elem #u128 (mk_u128 0) l in
+  let commhi:Alloc.Vec.t_Vec t_Commitment Alloc.Alloc.t_Global =
+    Alloc.Vec.impl__with_capacity #t_Commitment l
+  in
+  let commhi, hi:(Alloc.Vec.t_Vec t_Commitment Alloc.Alloc.t_Global &
+    Alloc.Vec.t_Vec u128 Alloc.Alloc.t_Global) =
+    Rust_primitives.Hax.Folds.fold_range (mk_usize 0)
+      l
+      (fun temp_0_ ll ->
+          let commhi, hi:(Alloc.Vec.t_Vec t_Commitment Alloc.Alloc.t_Global &
+            Alloc.Vec.t_Vec u128 Alloc.Alloc.t_Global) =
+            temp_0_
+          in
+          let ll:usize = ll in
+          b2t
+          (((Alloc.Vec.impl_1__len #u128 #Alloc.Alloc.t_Global hi <: usize) =. l <: bool) &&
+            ((Alloc.Vec.impl_1__len #t_Commitment #Alloc.Alloc.t_Global commhi <: usize) =. ll
+              <:
+              bool)) /\
+          b2t
+          ((Alloc.Vec.impl_1__len #Polytune.Data_types.t_Share #Alloc.Alloc.t_Global zshares
+              <:
+              usize) >=.
+            l
+            <:
+            bool) /\
+          (forall (ll: usize).
+              b2t
+              ((mk_usize 0 <=. ll <: bool) && (ll <. l <: bool) &&
+                ((Alloc.Vec.impl_1__len #Polytune.Data_types.t_Share #Alloc.Alloc.t_Global zshares
+                    <:
+                    usize) >=.
+                  l
+                  <:
+                  bool)) ==>
+              b2t
+              ((Alloc.Vec.impl_1__len #(Polytune.Data_types.t_Mac & Polytune.Data_types.t_Key)
+                    #Alloc.Alloc.t_Global
+                    (zshares.[ ll ] <: Polytune.Data_types.t_Share).Polytune.Data_types._1
+                      .Polytune.Data_types._0
+                  <:
+                  usize) >=.
+                n
+                <:
+                bool)))
+      (commhi, hi
+        <:
+        (Alloc.Vec.t_Vec t_Commitment Alloc.Alloc.t_Global &
+          Alloc.Vec.t_Vec u128 Alloc.Alloc.t_Global))
+      (fun temp_0_ ll ->
+          let commhi, hi:(Alloc.Vec.t_Vec t_Commitment Alloc.Alloc.t_Global &
+            Alloc.Vec.t_Vec u128 Alloc.Alloc.t_Global) =
+            temp_0_
+          in
+          let ll:usize = ll in
+          let hi:Alloc.Vec.t_Vec u128 Alloc.Alloc.t_Global =
+            Rust_primitives.Hax.Folds.fold_range (mk_usize 0)
+              n
+              (fun hi temp_1_ ->
+                  let hi:Alloc.Vec.t_Vec u128 Alloc.Alloc.t_Global = hi in
+                  let _:usize = temp_1_ in
+                  b2t
+                  (((Alloc.Vec.impl_1__len #u128 #Alloc.Alloc.t_Global hi <: usize) =. l <: bool) &&
+                    ((Alloc.Vec.impl_1__len #t_Commitment #Alloc.Alloc.t_Global commhi <: usize) =.
+                      ll
+                      <:
+                      bool)) /\
+                  b2t
+                  ((Alloc.Vec.impl_1__len #Polytune.Data_types.t_Share #Alloc.Alloc.t_Global zshares
+                      <:
+                      usize) >=.
+                    l
+                    <:
+                    bool) /\
+                  (forall (ll: usize).
+                      b2t
+                      ((mk_usize 0 <=. ll <: bool) && (ll <. l <: bool) &&
+                        ((Alloc.Vec.impl_1__len #Polytune.Data_types.t_Share
+                              #Alloc.Alloc.t_Global
+                              zshares
+                            <:
+                            usize) >=.
+                          l
+                          <:
+                          bool)) ==>
+                      b2t
+                      ((Alloc.Vec.impl_1__len #(Polytune.Data_types.t_Mac &
+                              Polytune.Data_types.t_Key)
+                            #Alloc.Alloc.t_Global
+                            (zshares.[ ll ] <: Polytune.Data_types.t_Share).Polytune.Data_types._1
+                              .Polytune.Data_types._0
+                          <:
+                          usize) >=.
+                        n
+                        <:
+                        bool)))
+              hi
+              (fun hi k ->
+                  let hi:Alloc.Vec.t_Vec u128 Alloc.Alloc.t_Global = hi in
+                  let k:usize = k in
+                  if k =. i <: bool
+                  then hi
+                  else
+                    let mk_zi, ki_zk:(Polytune.Data_types.t_Mac & Polytune.Data_types.t_Key) =
+                      (zshares.[ ll ] <: Polytune.Data_types.t_Share).Polytune.Data_types._1
+                        .Polytune.Data_types._0.[ k ]
+                    in
+                    Rust_primitives.Hax.Monomorphized_update_at.update_at_usize hi
+                      ll
+                      ((((hi.[ ll ] <: u128) ^. mk_zi.Polytune.Data_types._0 <: u128) ^.
+                          ki_zk.Polytune.Data_types._0
+                          <:
+                          u128) ^.
+                        ((ki_xj_phi.[ k ] <: Alloc.Vec.t_Vec u128 Alloc.Alloc.t_Global).[ ll ]
+                          <:
+                          u128)
+                        <:
+                        u128))
+          in
+          let hi:Alloc.Vec.t_Vec u128 Alloc.Alloc.t_Global =
+            Rust_primitives.Hax.Monomorphized_update_at.update_at_usize hi
+              ll
+              (((hi.[ ll ] <: u128) ^.
+                  ((cast ((xshares.[ ll ] <: Polytune.Data_types.t_Share).Polytune.Data_types._0
+                          <:
+                          bool)
+                      <:
+                      u128) *!
+                    (phi.[ ll ] <: u128)
+                    <:
+                    u128)
+                  <:
+                  u128) ^.
+                ((cast ((zshares.[ ll ] <: Polytune.Data_types.t_Share).Polytune.Data_types._0
+                        <:
+                        bool)
+                    <:
+                    u128) *!
+                  delta.Polytune.Data_types._0
+                  <:
+                  u128)
+                <:
+                u128)
+          in
+          let commhi:Alloc.Vec.t_Vec t_Commitment Alloc.Alloc.t_Global =
+            Alloc.Vec.impl_1__push #t_Commitment
+              #Alloc.Alloc.t_Global
+              commhi
+              (commit (Core.Num.impl_u128__to_be_bytes (hi.[ ll ] <: u128) <: t_Slice u8)
+                <:
+                t_Commitment)
+          in
+          commhi, hi
+          <:
+          (Alloc.Vec.t_Vec t_Commitment Alloc.Alloc.t_Global &
+            Alloc.Vec.t_Vec u128 Alloc.Alloc.t_Global))
+  in
+  let hax_temp_output:Core.Result.t_Result
+    (Alloc.Vec.t_Vec t_Commitment Alloc.Alloc.t_Global & Alloc.Vec.t_Vec u128 Alloc.Alloc.t_Global)
+    t_Error =
+    Core.Result.Result_Ok
+    (commhi, hi
+      <:
+      (Alloc.Vec.t_Vec t_Commitment Alloc.Alloc.t_Global & Alloc.Vec.t_Vec u128 Alloc.Alloc.t_Global
+      ))
+    <:
+    Core.Result.t_Result
+      (Alloc.Vec.t_Vec t_Commitment Alloc.Alloc.t_Global & Alloc.Vec.t_Vec u128 Alloc.Alloc.t_Global
+      ) t_Error
+  in
+  ki_xj_phi, zshares, hax_temp_output
+  <:
+  (Alloc.Vec.t_Vec (Alloc.Vec.t_Vec u128 Alloc.Alloc.t_Global) Alloc.Alloc.t_Global &
+    Alloc.Vec.t_Vec Polytune.Data_types.t_Share Alloc.Alloc.t_Global &
+    Core.Result.t_Result
+      (Alloc.Vec.t_Vec t_Commitment Alloc.Alloc.t_Global & Alloc.Vec.t_Vec u128 Alloc.Alloc.t_Global
+      ) t_Error)
+
+let flaand_3_
+      (i n l: usize)
+      (xor_all_hi: Alloc.Vec.t_Vec u128 Alloc.Alloc.t_Global)
+      (commhi_k:
+          Alloc.Vec.t_Vec (Alloc.Vec.t_Vec t_Commitment Alloc.Alloc.t_Global) Alloc.Alloc.t_Global)
+      (hi_k_outer: Alloc.Vec.t_Vec (Alloc.Vec.t_Vec u128 Alloc.Alloc.t_Global) Alloc.Alloc.t_Global)
+    : Prims.Pure (Core.Result.t_Result Prims.unit t_Error)
+      (requires
+        b2t ((Alloc.Vec.impl_1__len #u128 #Alloc.Alloc.t_Global xor_all_hi <: usize) =. l <: bool) /\
+        b2t
+        ((Alloc.Vec.impl_1__len #(Alloc.Vec.t_Vec t_Commitment Alloc.Alloc.t_Global)
+              #Alloc.Alloc.t_Global
+              commhi_k
+            <:
+            usize) >=.
+          n
+          <:
+          bool) /\
+        (forall (k: usize).
+            b2t
+            ((mk_usize 0 <=. k <: bool) && (k <. n <: bool) &&
+              ((Alloc.Vec.impl_1__len #(Alloc.Vec.t_Vec t_Commitment Alloc.Alloc.t_Global)
+                    #Alloc.Alloc.t_Global
+                    commhi_k
+                  <:
+                  usize) >=.
+                n
+                <:
+                bool)) ==>
+            b2t
+            ((Alloc.Vec.impl_1__len #t_Commitment
+                  #Alloc.Alloc.t_Global
+                  (commhi_k.[ k ] <: Alloc.Vec.t_Vec t_Commitment Alloc.Alloc.t_Global)
+                <:
+                usize) >=.
+              l
+              <:
+              bool)) /\
+        (b2t
+        ((Alloc.Vec.impl_1__len #(Alloc.Vec.t_Vec u128 Alloc.Alloc.t_Global)
+              #Alloc.Alloc.t_Global
+              hi_k_outer
+            <:
+            usize) >=.
+          n
+          <:
+          bool) /\
+        (forall (k: usize).
+            b2t
+            ((mk_usize 0 <=. k <: bool) && (k <. n <: bool) &&
+              ((Alloc.Vec.impl_1__len #(Alloc.Vec.t_Vec u128 Alloc.Alloc.t_Global)
+                    #Alloc.Alloc.t_Global
+                    hi_k_outer
+                  <:
+                  usize) >=.
+                n
+                <:
+                bool)) ==>
+            b2t
+            ((Alloc.Vec.impl_1__len #u128
+                  #Alloc.Alloc.t_Global
+                  (hi_k_outer.[ k ] <: Alloc.Vec.t_Vec u128 Alloc.Alloc.t_Global)
+                <:
+                usize) >=.
+              l
+              <:
+              bool))))
+      (fun _ -> Prims.l_True) =
+  let commitment_error:bool = false in
+  let xor_not_zero_error:bool = false in
+  let commitment_error, xor_all_hi:(bool & Alloc.Vec.t_Vec u128 Alloc.Alloc.t_Global) =
+    Rust_primitives.Hax.Folds.fold_range (mk_usize 0)
+      n
+      (fun temp_0_ temp_1_ ->
+          let commitment_error, xor_all_hi:(bool & Alloc.Vec.t_Vec u128 Alloc.Alloc.t_Global) =
+            temp_0_
+          in
+          let _:usize = temp_1_ in
+          (Alloc.Vec.impl_1__len #u128 #Alloc.Alloc.t_Global xor_all_hi <: usize) =. l <: bool)
+      (commitment_error, xor_all_hi <: (bool & Alloc.Vec.t_Vec u128 Alloc.Alloc.t_Global))
+      (fun temp_0_ k ->
+          let commitment_error, xor_all_hi:(bool & Alloc.Vec.t_Vec u128 Alloc.Alloc.t_Global) =
+            temp_0_
+          in
+          let k:usize = k in
+          if k =. i <: bool
+          then commitment_error, xor_all_hi <: (bool & Alloc.Vec.t_Vec u128 Alloc.Alloc.t_Global)
+          else
+            Rust_primitives.Hax.Folds.fold_range (mk_usize 0)
+              l
+              (fun temp_0_ temp_1_ ->
+                  let commitment_error, xor_all_hi:(bool & Alloc.Vec.t_Vec u128 Alloc.Alloc.t_Global
+                  ) =
+                    temp_0_
+                  in
+                  let _:usize = temp_1_ in
+                  (Alloc.Vec.impl_1__len #u128 #Alloc.Alloc.t_Global xor_all_hi <: usize) =. l
+                  <:
+                  bool)
+              (commitment_error, xor_all_hi <: (bool & Alloc.Vec.t_Vec u128 Alloc.Alloc.t_Global))
+              (fun temp_0_ ll ->
+                  let commitment_error, xor_all_hi:(bool & Alloc.Vec.t_Vec u128 Alloc.Alloc.t_Global
+                  ) =
+                    temp_0_
+                  in
+                  let ll:usize = ll in
+                  let commitment_error:bool =
+                    if
+                      ~.(open_commitment ((commhi_k.[ k ]
+                              <:
+                              Alloc.Vec.t_Vec t_Commitment Alloc.Alloc.t_Global).[ ll ]
+                            <:
+                            t_Commitment)
+                          (Core.Num.impl_u128__to_be_bytes ((hi_k_outer.[ k ]
+                                  <:
+                                  Alloc.Vec.t_Vec u128 Alloc.Alloc.t_Global).[ ll ]
+                                <:
+                                u128)
+                            <:
+                            t_Slice u8)
+                        <:
+                        bool)
+                    then
+                      let commitment_error:bool = true in
+                      commitment_error
+                    else commitment_error
+                  in
+                  let xor_all_hi:Alloc.Vec.t_Vec u128 Alloc.Alloc.t_Global =
+                    Rust_primitives.Hax.Monomorphized_update_at.update_at_usize xor_all_hi
+                      ll
+                      ((xor_all_hi.[ ll ] <: u128) ^.
+                        ((hi_k_outer.[ k ] <: Alloc.Vec.t_Vec u128 Alloc.Alloc.t_Global).[ ll ]
+                          <:
+                          u128)
+                        <:
+                        u128)
+                  in
+                  commitment_error, xor_all_hi <: (bool & Alloc.Vec.t_Vec u128 Alloc.Alloc.t_Global)
+              )
+            <:
+            (bool & Alloc.Vec.t_Vec u128 Alloc.Alloc.t_Global))
+  in
+  let xor_not_zero_error:bool =
+    Rust_primitives.Hax.Folds.fold_range (mk_usize 0)
+      l
+      (fun xor_not_zero_error temp_1_ ->
+          let xor_not_zero_error:bool = xor_not_zero_error in
+          let _:usize = temp_1_ in
+          (Alloc.Vec.impl_1__len #u128 #Alloc.Alloc.t_Global xor_all_hi <: usize) =. l <: bool)
+      xor_not_zero_error
+      (fun xor_not_zero_error i ->
+          let xor_not_zero_error:bool = xor_not_zero_error in
+          let i:usize = i in
+          if (xor_all_hi.[ i ] <: u128) <>. mk_u128 0 <: bool
+          then
+            let xor_not_zero_error:bool = true in
+            xor_not_zero_error
+          else xor_not_zero_error)
+  in
+  if commitment_error
+  then
+    Core.Result.Result_Err (Error_CommitmentCouldNotBeOpened <: t_Error)
+    <:
+    Core.Result.t_Result Prims.unit t_Error
+  else
+    if xor_not_zero_error
+    then
+      Core.Result.Result_Err (Error_LaANDXorNotZero <: t_Error)
+      <:
+      Core.Result.t_Result Prims.unit t_Error
+    else Core.Result.Result_Ok (() <: Prims.unit) <: Core.Result.t_Result Prims.unit t_Error
 
 /// Combine two leaky ANDs into one non-leaky AND.
 let combine_two_leaky_ands (i n: usize) (x1 y1 z1 x2 z2: Polytune.Data_types.t_Share) (d: bool)
