e.sh
@@ -10,5 +10,5 @@ rm -f proofs/fstar/extraction/Polytune.*
 # rm -rf proofs/fstar/extraction/.depend 
 
 ./hax-driver.py extract-fstar
-# sed -i 's/((ei_uij_k\.\[ j \] <: Alloc\.Vec\.t_Vec (bool & u128) Alloc\.Alloc\.t_Global)\.\[ ll \])/((ei_uij_k.[ j ] <: Alloc.Vec.t_Vec (bool \& u128) Alloc.Alloc.t_Global).[ ll ] <: (bool \& u128))/' ./proofs/fstar/extraction/Polytune.Faand.fst 
+sed -i 's/((ei_uij_k\.\[ j \] <: Alloc\.Vec\.t_Vec (bool & u128) Alloc\.Alloc\.t_Global)\.\[ ll \])/((ei_uij_k.[ j ] <: Alloc.Vec.t_Vec (bool \& u128) Alloc.Alloc.t_Global).[ ll ] <: (bool \& u128))/' ./proofs/fstar/extraction/Polytune.Faand.fst 
 ./hax-driver.py typecheck-fstar
